mutable context in VCGen

src/Semantics/Semantics1.dfy
@@ -31,18 +31,23 @@
       case Var(v) => {v}
     }
 
-    predicate DefinedOn(s: State) {
-      forall v <- FVars() :: v in s.Keys
+    predicate IsDefinedOn(s: set<Variable>) {
+      forall v <- FVars() :: v in s
     }
 
+    // TODO: make a Dafny issue (check if there already is one)
     ghost predicate Holds() {
-      forall s: State :: DefinedOn(s) ==> s.Eval(this)
+      forall s: State :: IsDefinedOn(s.Keys) ==> s.Eval(this)
     }
   }
 
   function Eq(e1: Expr, e2: Expr): Expr {
     And(Implies(e1, e2), Implies(e2, e1))
   }
+
+  lemma FVarsEqLemma(e1: Expr, e2: Expr)
+    ensures Eq(e1, e2).FVars() == e1.FVars() + e2.FVars()
+  {  }
     
   datatype Stmt =
     | Check(e: Expr)
@@ -58,10 +63,10 @@
         case Check(e) => e.FVars()
         case Assume(e) => e.FVars()
         case Seq(s0, s1) => s0.FVars() + s1.FVars()
-        case Assign(lhs, rhs) => rhs.FVars()
+        case Assign(lhs, rhs) => {lhs} + rhs.FVars()
       }
-      predicate DefinedOn(s: State) {
-        forall v <- FVars() :: v in s.Keys
+      predicate IsDefinedOn(s: set<Variable>) {
+        forall v <- FVars() :: v in s
       }
     }
 
@@ -71,7 +76,7 @@
     
   // datatype State = State(m: map<string, Value>) {
     function Eval(e: Expr): Value 
-      requires e.DefinedOn(this)
+      requires e.IsDefinedOn(this.Keys)
       decreases e
     {
       match e
@@ -113,22 +118,22 @@
   {
     match s
     case Check(e) =>
-      e.DefinedOn(a) &&
+      e.IsDefinedOn(a.Keys) &&
       z == if a.Eval(e) then Ok(a) else Error
     case Assume(e) =>
-      e.DefinedOn(a) &&
+      e.IsDefinedOn(a.Keys) &&
       a.Eval(e) && z == Ok(a)
     case Seq(s0, s1) =>
       exists w ::
         && BigStep(s0, a, w) 
         && match w {
             case Ok(b) => 
-              && s1.DefinedOn(b) 
+              && s1.IsDefinedOn(b.Keys) 
               && BigStep(s1, b, z)
             case _ => z == w
         }
     case Assign(lhs, rhs) =>
-      && rhs.DefinedOn(a) 
+      && rhs.IsDefinedOn(a.Keys) 
       && a.Eval(rhs) 
       && z == Ok(a.Update(lhs, a.Eval(rhs)))
     // case While(guard, inv, body) =>
@@ -142,10 +147,25 @@
     //     BigStep(els, a, z)
   }
 
-    function Conj(ctx: seq<Expr>): Expr 
-    {
-      if ctx == [] then BConst(true) else And(ctx[0], Conj(ctx[1..]))
+  function Conj(ctx: seq<Expr>): Expr 
+  {
+    if ctx == [] then BConst(true) else And(ctx[0], Conj(ctx[1..]))
+  }
+
+
+  lemma FVarsConjUnionLemma(ctx1: seq<Expr>, ctx2: seq<Expr>)
+    ensures Conj(ctx1 + ctx2).FVars() == Conj(ctx1).FVars() + Conj(ctx2).FVars()
+  {
+    if ctx1 == [] {
+      assert [] + ctx2 == ctx2; // if I remove this everything breaks
+    } else {
+      assert ctx1 + ctx2 == [ctx1[0]] + (ctx1[1..] + ctx2);
     }
+  }
+
+  // lemma FVarsConjSingleLemma(e: Expr)
+  //   ensures Conj([e]).FVars() == e.FVars()
+  // {  }
 
   class Context {
     var ctx: seq<Expr>
@@ -161,18 +181,22 @@
       ctx := [];
       incarnation := map[];
     }
-    // Q: How to prove that `v !in incarnation.Keys` is satisfiable?
+
+    // How to prove that `v !in incarnation.Keys` is satisfiable?
     method FreshVar() returns (v: Variable) 
-      ensures {:axiom} v !in incarnation.Keys
-    // {
-    //     // assert !incarnation.Keys != {};
-    //     // assert {:axiom} exists v :: v !in incarnation.Keys;
-    //     // var u :| v !in incarnation.Keys;
-    //     // v := u;
-    // }
+      ensures v !in incarnation.Keys
+    {
+        // assert !incarnation.Keys != {};
+        // assert {:axiom} exists v :: v !in incarnation.Keys;
+        v :| v !in incarnation.Keys by {
+          // Prove existence here
+          assume {:axiom} false;
+          // loop increasing length
+        }
+    }
 
     function Substitute(e: Expr): Expr 
-      reads this
+      reads `incarnation
     {
       match e
       case Var(v) =>
@@ -191,13 +215,14 @@
     }
 
     function SubstituteStmt(s: Stmt): Stmt 
+      requires s.IsDefinedOn(incarnation.Keys)
       reads this
     {
       match s
       case Check(e) => Check(Substitute(e))
       case Assume(e) => Assume(Substitute(e))
       case Seq(s0, s1) => Seq(SubstituteStmt(s0), SubstituteStmt(s1))
-      case Assign(lhs, rhs) => Assign(lhs, Substitute(rhs))
+      case Assign(lhs, rhs) => Assign(incarnation[lhs], Substitute(rhs))
     }
 
     function MkEntailment(e: Expr): Expr 
@@ -206,39 +231,60 @@
       Implies(Conj(ctx), Substitute(e))
     }
 
+    lemma SeqAppendLemma(x: seq<Expr>, y: seq<Expr>)
+      ensures y <= x + y
+    {
+      if x == [] {
+      } else {
+
+      }
+    }
+
     method Add(e: Expr) 
+      requires Valid()
+      ensures Valid()
+      ensures incarnation == old(incarnation)
+      ensures old(ctx) <= ctx
       modifies this
     {
       ctx := [Substitute(e)] + ctx;
+      SeqAppendLemma([Substitute(e)], old(ctx));
     }
 
     method AddEq(v: Variable, e: Expr) 
+      requires v in incarnation.Keys
+      requires Valid()
+      ensures Valid()
+      ensures old(ctx) <= ctx
+      ensures incarnation.Keys == old(incarnation.Keys)
       modifies this
     {
       var vNew := FreshVar();
-      var eNew := Substitute(e);
+      ctx := [Eq(Var(vNew), Substitute(e))] + ctx;
+      FVarsEqLemma(Var(vNew), Substitute(e));
       incarnation := incarnation[v := vNew];
-      Add(Eq(Var(vNew), eNew));
+      SeqAppendLemma([Substitute(e)], old(ctx));
     }
 
-    ghost predicate DefinedOn(s: State) 
+    ghost predicate IsDefinedOn(s: set<Variable>) 
       reads this
     {
-      forall e <- ctx :: e.DefinedOn(s)
+      forall e <- ctx :: e.IsDefinedOn(s)
     }
 
-    ghost predicate IsModeled(s: State) 
+    ghost predicate IsSatisfiedOn(s: State) 
       reads this
     {
-      DefinedOn(s) && forall e <- ctx :: s.Eval(e)
+      IsDefinedOn(s.Keys) && forall e <- ctx :: s.Eval(e)
     }
 
     ghost predicate Entails(e: Expr) 
       reads this
     {
       forall s: State ::  
-        e.DefinedOn(s) && IsModeled(s) ==> s.Eval(e)
+        e.IsDefinedOn(s.Keys) && IsSatisfiedOn(s) ==> s.Eval(e)
     }
+
   lemma FVarsSubsituteLemma(e: Expr)
     ensures Substitute(e).FVars() <= e.FVars() + incarnation.Values
   {  }
@@ -246,24 +292,21 @@
 
 
 
-  lemma DefinedOnAndLemma(e0: Expr, e1: Expr, s: State)
-    requires e0.DefinedOn(s) && e1.DefinedOn(s)
-    ensures And(e0, e1).DefinedOn(s) { }
+  lemma IsDefinedOnAndLemma(e0: Expr, e1: Expr, s: State)
+    requires e0.IsDefinedOn(s.Keys) && e1.IsDefinedOn(s.Keys)
+    ensures And(e0, e1).IsDefinedOn(s.Keys) { }
 
-  lemma DefinedOnConjLemma(ctx: seq<Expr>, s: State)
-    requires forall e <- ctx :: e.DefinedOn(s)
-    ensures Conj(ctx).DefinedOn(s)
+  lemma IsDefinedOnConjLemma(ctx: seq<Expr>, s: State)
+    requires forall e <- ctx :: e.IsDefinedOn(s.Keys)
+    ensures Conj(ctx).IsDefinedOn(s.Keys)
     {
-      if ctx != [] { DefinedOnAndLemma(ctx[0], Conj(ctx[1..]), s); }
+      if ctx != [] { IsDefinedOnAndLemma(ctx[0], Conj(ctx[1..]), s); }
     }
-
-  // Q: How to get rid of one of the pre conditions?
-  // they are equivalent, but one is needed for Eval in 1 and the other in 2
   lemma EvalConjLemma(ctx: seq<Expr>, s: State)
-    requires Conj(ctx).DefinedOn(s)
-    requires forall e <- ctx :: e.DefinedOn(s)
+    // requires Conj(ctx).IsDefinedOn(s.Keys)
+    requires forall e <- ctx :: e.IsDefinedOn(s.Keys)
     requires forall e <- ctx :: s.Eval(e) // 1
-    ensures s.Eval(Conj(ctx))             // 2
+    ensures (IsDefinedOnConjLemma(ctx, s); s.Eval(Conj(ctx)))             // 2
   {  }
 
   lemma MkEntailmentLemma(e: Expr, context: Context)
@@ -271,29 +314,30 @@
     ensures 
       context.MkEntailment(e).Holds() ==> 
       forall s: State :: 
-        context.IsModeled(s) && context.Substitute(e).DefinedOn(s) ==> s.Eval(context.Substitute(e)) {
+        context.IsSatisfiedOn(s) && context.Substitute(e).IsDefinedOn(s.Keys) ==> s.Eval(context.Substitute(e)) {
       if context.MkEntailment(e).Holds() {
-        forall s: State | context.IsModeled(s) && context.Substitute(e).DefinedOn(s)
+        forall s: State | context.IsSatisfiedOn(s) && context.Substitute(e).IsDefinedOn(s.Keys)
           ensures s.Eval(context.Substitute(e)) {
-            DefinedOnConjLemma(context.ctx, s);
+            IsDefinedOnConjLemma(context.ctx, s);
             context.FVarsSubsituteLemma(e);
-            assert context.MkEntailment(e).DefinedOn(s);
+            assert context.MkEntailment(e).IsDefinedOn(s.Keys);
             EvalConjLemma(context.ctx, s);
       }
     }
   }
 
-
-  method VCGenAux(s: Stmt, context: Context) 
-  returns (result: set<Expr>) 
-  requires context.Valid()
-  requires s.Check? || s.Assume?
-  ensures context.Valid()
-  ensures 
-    (forall e <- result :: e.Holds()) ==> 
-      forall st: State, out: Except<State> :: 
-        context.IsModeled(st) ==>
-        BigStep(context.SubstituteStmt(s), st, out) ==> out.Ok?
+method VCGenAux(s: Stmt, context: Context) returns (result: set<Expr>) 
+    requires context.Valid()
+    requires s.IsDefinedOn(context.incarnation.Keys)
+    ensures context.Valid()
+    ensures old(context.incarnation.Keys) == context.incarnation.Keys
+    ensures old(context.ctx) <= context.ctx
+    ensures 
+      (forall e <- result :: e.Holds()) ==> 
+        forall st: State, out: Except<State> :: 
+          // Q: why old(context).IsSatisfiedOn(st) does not work?
+          old(context.IsSatisfiedOn(st)) ==>
+          BigStep(old(context.SubstituteStmt(s)), st, out) ==> out.Ok?
     modifies context
   {
     match s
@@ -303,13 +347,84 @@
     case Assume(e) =>
       context.Add(e);
       result := {};
-    // case Seq(s0, s1) =>
-    //   var r0 := VCGenAux(s0, context);
-    //   var r1 := VCGenAux(s1, context);
-    //   result := r0 + r1;
-    // case Assign(lhs, rhs) =>
-    //   context.AddEq(lhs, rhs);
-    //   result := {};
+    case Assign(lhs, rhs) =>
+      context.AddEq(lhs, rhs);
+      result := {};
+    case Seq(s0, s1) =>
+      // assume {:axiom} false;
+      var r0 := VCGenAux(s0, context);
+      ghost var ctx := context.ctx;
+      var r1 := VCGenAux(s1, context);
+      assert ctx <= context.ctx;
+      assert 
+        (forall e <- r0 :: e.Holds()) ==> 
+          forall st: State, out: Except<State> :: 
+            old(context.IsSatisfiedOn(st)) ==>
+            BigStep(old(context.SubstituteStmt(s0)), st, out) ==> out.Ok?;
+      assert 
+        (forall e <- r0 :: e.Holds()) ==> 
+          forall st: State, out: Except<State> :: 
+            old(context.IsSatisfiedOn(st)) ==>
+            BigStep(old(context.SubstituteStmt(s0)), st, out) ==> out.Ok?;
+      result := r0 + r1;
+    // case While(guard, inv, body) =>
+    //   var invIn := context.MkEntailment(inv);
+
+      // var ctxInv := new Context();
+      // ctxInv.Add(inv);
+
+      // var invMid := VCGenAux(body, ctxInv);
+      // var invPreserve := ctxInv.MkEntailment(inv);
+      // result := {invIn} + invMid + {invPreserve};
+      
+    // case If(cond, thn, els) => result := {BConst(false)}; // what happens here?
+      // var ctx := context;
+      // var r0 := VCGenAux(thn, ctx);
+      // var r1 := VCGenAux(els, ctx);
+      // result := r0 + r1;
+  }
+
+  method VCGenAux(s: Stmt, context: Context) returns (result: set<Expr>) 
+    requires context.Valid()
+    requires s.IsDefinedOn(context.incarnation.Keys)
+    ensures context.Valid()
+    ensures old(context.incarnation.Keys) == context.incarnation.Keys
+    ensures old(context.ctx) <= context.ctx
+    ensures 
+      (forall e <- result :: e.Holds()) ==> 
+        forall st: State, out: Except<State> :: 
+          // Q: why old(context).IsSatisfiedOn(st) does not work?
+          old(context.IsSatisfiedOn(st)) ==>
+          BigStep(old(context.SubstituteStmt(s)), st, out) ==> out.Ok?
+    modifies context
+  {
+    match s
+    case Check(e) =>
+      result := {context.MkEntailment(e)};
+      MkEntailmentLemma(e, context);
+    case Assume(e) =>
+      context.Add(e);
+      result := {};
+    case Assign(lhs, rhs) =>
+      context.AddEq(lhs, rhs);
+      result := {};
+    case Seq(s0, s1) =>
+      // assume {:axiom} false;
+      var r0 := VCGenAux(s0, context);
+      ghost var ctx := context.ctx;
+      var r1 := VCGenAux(s1, context);
+      assert ctx <= context.ctx;
+      assert 
+        (forall e <- r0 :: e.Holds()) ==> 
+          forall st: State, out: Except<State> :: 
+            old(context.IsSatisfiedOn(st)) ==>
+            BigStep(old(context.SubstituteStmt(s0)), st, out) ==> out.Ok?;
+      assert 
+        (forall e <- r0 :: e.Holds()) ==> 
+          forall st: State, out: Except<State> :: 
+            old(context.IsSatisfiedOn(st)) ==>
+            BigStep(old(context.SubstituteStmt(s0)), st, out) ==> out.Ok?;
+      result := r0 + r1;
     // case While(guard, inv, body) =>
     //   var invIn := context.MkEntailment(inv);
 
